First attempt at flatten iterator

Flatten_Iter.thy
@@ -1,24 +1,152 @@
 theory Flatten_Iter
-imports Basic_Assn
+  imports
+  Basic_Assn
+  "Separation_Logic_Imperative_HOL.Imp_List_Spec"
+  "HOL-Real_Asymp.Inst_Existentials"
 begin
 
-locale imp_list_iterate = 
-  constrains is_list :: "'a list \<Rightarrow> 'l \<Rightarrow> assn"
-  fixes is_it :: "'a list \<Rightarrow> 'l \<Rightarrow> 'a list \<Rightarrow> 'it \<Rightarrow> assn"
-  fixes it_init :: "'l \<Rightarrow> ('it) Heap"
-  fixes it_has_next :: "'it \<Rightarrow> bool Heap"
-  fixes it_next :: "'it \<Rightarrow> ('a\<times>'it) Heap"
-  assumes it_init_rule[sep_heap_rules]: 
-    "<is_list l p> it_init p <is_it l p l>\<^sub>t"
-  assumes it_next_rule[sep_heap_rules]: "l'\<noteq>[] \<Longrightarrow> 
-    <is_it l p l' it> 
-      it_next it 
-    <\<lambda>(a,it'). is_it l p (tl l') it' * \<up>(a=hd l')>"
-  assumes it_has_next_rule[sep_heap_rules]: 
-    "<is_it l p l' it> 
-       it_has_next it 
-     <\<lambda>r. is_it l p l' it * \<up>(r\<longleftrightarrow>l'\<noteq>[])>"
-  assumes quit_iteration:
-    "is_it l p l' it \<Longrightarrow>\<^sub>A is_list l p * true"
+text "This locale takes an iterator that refines a list of elements that themselves
+can be iterated and defines an iterator over the flattened list of lower level elements"
+
+locale flatten_iter =
+  inner_list: imp_list_iterate is_inner_list inner_is_it inner_it_init inner_it_has_next inner_it_next + 
+  outer_list: imp_list_iterate is_outer_list outer_is_it outer_it_init outer_it_has_next outer_it_next 
+  for is_outer_list :: "'l list \<Rightarrow> 'm \<Rightarrow> assn"
+  and outer_is_it :: "'l list \<Rightarrow> 'm \<Rightarrow> 'l list \<Rightarrow> 'oit \<Rightarrow> assn"
+  and outer_it_init :: "'m \<Rightarrow> ('oit) Heap"
+  and outer_it_has_next :: "'oit \<Rightarrow> bool Heap"
+  and outer_it_next :: "'oit \<Rightarrow> ('l\<times>'oit) Heap"
+  and is_inner_list :: "'a list \<Rightarrow> 'l \<Rightarrow> assn"
+  and inner_is_it :: "'a list \<Rightarrow> 'l \<Rightarrow> 'a list \<Rightarrow> 'iit \<Rightarrow> assn"
+  and inner_it_init :: "'l \<Rightarrow> ('iit) Heap"
+  and inner_it_has_next :: "'iit \<Rightarrow> bool Heap"
+  and inner_it_next :: "'iit \<Rightarrow> ('a\<times>'iit) Heap"
+begin
+
+fun is_flatten_list :: "'a list \<Rightarrow> 'm \<Rightarrow> assn" where
+  "is_flatten_list ls lsi = (\<exists>\<^sub>A lsi' ls'.
+    is_outer_list lsi' lsi * list_assn is_inner_list ls' lsi' * \<up>(ls = concat ls')
+)"
+
+(*type_synonym flatten_it = "'iit \<times> 'oit"*)
+fun is_flatten_it :: "'a list \<Rightarrow> 'm \<Rightarrow> 'a list \<Rightarrow> ('oit \<times> 'iit option) \<Rightarrow> assn"
+  where 
+"is_flatten_it ls lsi ls2 (oit, None) = 
+        (\<exists>\<^sub>A lsi' ls2' ls1' lsi1 lsi2.
+          list_assn is_inner_list ls1' lsi1 *
+          list_assn is_inner_list ls2' lsi2 *
+           \<up>(ls2 = concat ls2' \<and> ls = (concat (ls1'@ls2'))) *
+          outer_is_it lsi' lsi lsi2 oit *
+          \<up>(lsi'=lsi1@lsi2)
+)" |
+"is_flatten_it ls lsi ls2 (oit, Some iit) = 
+        (\<exists>\<^sub>A lsi' ls2' ls1' lsi1 lsi2 lsim ls2m lsm ls1m.
+          list_assn is_inner_list ls1' lsi1 *
+          list_assn is_inner_list ls2' lsi2 *
+           \<up>(ls2m \<noteq> [] \<and> ls2 = ls2m@(concat ls2') \<and> ls = (concat (ls1'@lsm#ls2'))) *
+          outer_is_it lsi' lsi lsi2 oit *
+          \<up>(lsm = ls1m@ls2m \<and> lsi'=(lsi1@lsim#lsi2)) *
+          inner_is_it lsm lsim ls2m iit
+)
+"
+
+partial_function (heap) flatten_it_adjust:: "'oit \<Rightarrow> 'iit \<Rightarrow> ('oit \<times> 'iit option) Heap" where
+"flatten_it_adjust oit iit = do {
+      ihasnext \<leftarrow> inner_it_has_next iit;
+      if ihasnext then
+        return (oit, Some iit)
+      else do {
+        ohasnext \<leftarrow> outer_it_has_next oit;
+        if \<not>ohasnext then
+          return (oit, None)
+        else do {
+          (next, oit) \<leftarrow> outer_it_next oit;
+          nextit \<leftarrow> inner_it_init next;
+          flatten_it_adjust oit nextit
+        }
+      }
+  }
+"
+
+lemma flatten_it_adjust_rule: 
+  "lsm = lsm1@lsm2 \<Longrightarrow> 
+<list_assn is_inner_list ls1' ls1 * list_assn is_inner_list ls2' ls2 * outer_is_it (ls1@lsim#ls2) lsi ls2 oit * inner_is_it lsm lsim lsm2 iit>
+  flatten_it_adjust oit iit
+  <is_flatten_it (concat (ls1'@lsm#ls2')) lsi (concat (lsm2#ls2'))>\<^sub>t"
+  apply(subst flatten_it_adjust.simps)
+  apply (sep_auto eintros del: exI heap add: inner_list.it_has_next_rule)
+  apply(inst_existentials "(ls1 @ lsim # ls2)" ls2' ls1' ls1 ls2 lsim lsm2 lsm)
+  subgoal by auto
+  subgoal by (sep_auto)
+  apply (vcg (ss))
+  apply (vcg (ss))
+  apply (vcg (ss))
+  apply (vcg (ss))
+  apply (vcg (ss))
+  apply (vcg (ss))
+  apply (vcg (ss))
+  apply (vcg (ss))
+  apply (vcg (ss))
+  apply (vcg (ss))
+  apply (sep_auto eintros del: exI)
+  apply(inst_existentials "(ls1 @ [lsim])" "[lsm]" ls1' ls1 "[lsim]")
+  apply auto
+  apply(case_tac ls2; case_tac ls2')
+  apply (simp add: mult.left_assoc)+
+  apply (sep_auto eintros del: exI heap add: inner_list.it_init_rule)
+
+definition flatten_it_init :: "'m \<Rightarrow> _ Heap" 
+  where "flatten_it_init l = do {
+    oit \<leftarrow> outer_it_init l;
+    ohasnext \<leftarrow> outer_it_has_next oit;
+    if ohasnext then do {
+       (next, oit) \<leftarrow> outer_it_next oit;
+       nextit \<leftarrow> inner_it_init next;
+       flatten_it_adjust oit nextit
+    } else return (oit, None)
+}"
+
+lemma flatten_it_init_rule[sep_heap_rules]: 
+    "<is_flatten_list l p> flatten_it_init p <is_flatten_it l p l>\<^sub>t"
+  unfolding flatten_it_init_def
+  apply simp
+  find_theorems "<\<exists>\<^sub>A_._>_<_>"
+  apply(rule norm_pre_ex_rule)+
+  apply (vcg (ss))
+  apply (vcg (ss))
+  apply (vcg (ss))
+  apply (vcg (ss))
+  apply (vcg (ss))
+  apply (vcg (ss))
+  apply (vcg (ss))
+  apply (vcg (ss))
+  apply (vcg (ss))
+  apply (vcg (ss))
+  apply (vcg (ss))
+  apply (vcg (ss))
+  apply (vcg (ss))
+  apply (vcg (ss))
+  apply (vcg (ss))
+  apply (vcg (ss))
+  apply (vcg (ss))
+  apply (vcg (ss))
+  apply(case_tac lsi'; case_tac ls')
+  apply simp+
+  apply(rule impI)
+  thm inner_list.it_init_rule
+  apply (vcg heap add: inner_list.it_init_rule)
+
+definition flatten_it_next where 
+  "flatten_it_next \<equiv> \<lambda>(oit,iit). do {
+    (x, iit) \<leftarrow> inner_it_next iit;
+    (oit, iit) \<leftarrow> flatten_it_adjust oit iit;
+    return (x, (oit,iit))
+  }"
+
+definition flatten_it_has_next where
+  "flatten_it_has_next \<equiv> \<lambda>(oit, iit). do {
+    return (iit \<noteq> None)
+}"
+
 
 end
